feat: Build the k-induction circuit, but by building variables in Circuit for subterm sharing (#1334)
This is much easier to do than changing the whole data structure to AIG,
and should provide similar sharing of key circuits as the AIG encoding
does. While this does not provide *full* subcircuit sharing, it shares
"enough": It shares the computation of the state vector and the output,
which is the key construction that will prevent blowup of the circuit
size.

This is an alternative implementation strategy to #1330 , which requires
moving wholesale to AIGs. That's quite a drastic and deep change, and
would need more time to be robust.

SSA/Experimental/Bits/Fast/ReflectVerif.lean
@@ -394,39 +394,6 @@ def checkCircuitUnsatAux [DecidableEq α] [Hashable α] [Fintype α]
     | .ok cert => return .some cert
 
 
--- open Std Sat AIG Tactic BVDecide Frontend in
--- @[nospecialize]
--- def checkCircuitTautoAuxImpl
---     [DecidableEq α] [Hashable α] [Fintype α]
---     (c : Circuit α) : TermElabM (Option LratCert) := do
---   let cfg : BVDecideConfig := { timeout := cadicalTimeoutSec }
---   IO.FS.withTempFile fun _ lratFile => do
---     let cfg ← BVDecide.Frontend.TacticContext.new lratFile cfg
---     let c := ~~~ c -- we're checking TAUTO, so check that negation is UNSAT.
---     let entrypoint := c.toAIG
---     let ⟨entrypoint, _labelling⟩ := entrypoint.relabelNat'
---     let cnf := toCNF entrypoint
---     let out ← runExternal cnf cfg.solver cfg.lratPath
---       (trimProofs := true)
---       (timeout := cadicalTimeoutSec)
---       (binaryProofs := true)
---     match out with
---     | .error _model => return none
---     | .ok cert => return some cert
-
--- open Std Sat AIG Tactic BVDecide Frontend in
--- @[implemented_by checkCircuitTautoAuxImpl, nospecialize]
--- def checkCircuitTautoAux {α : Type}
---     [DecidableEq α] [Hashable α] [Fintype α]
---     (c : Circuit α) : TermElabM (Option LratCert) := do
---   return none
-
--- /--
--- An axiom that tracks that a theorem is true because of our currently unverified
--- 'decideIfZerosM' decision procedure.
--- -/
--- axiom decideIfZerosMAx {p : Prop} : p
-
 /--
 An inductive type representing the variables in the unrolled FSM circuit,
 where we unroll for 'n' steps.
@@ -438,6 +405,9 @@ deriving DecidableEq, Hashable
 
 
 namespace Inputs
+
+def elimEmpty {α : Sort u} (i : Inputs Empty i) : α :=
+  i.input.elim
 
 def elim0 {α : Sort u} (i : Inputs ι 0) : α :=
   i.ix.elim0
@@ -497,25 +467,62 @@ def format (f : ι → Format) (is : Inputs ι n) : Format :=
 
 end Inputs
 
+-- at 0:
+-- + free s0.
+
+-- at 1:
+-- + free s0
+-- --- x ---
+-- + o0 = evalWith(s0, i0).
+-- + s1 = carryWith(s0, i0)
+-- --- x ---
+
+-- at 2:
+-- + free s0
+-- --- x ---
+-- + o0 = evalWith(s0, i0).
+-- + s1 = carryWith(s0, i0)
+-- --- x ---
+-- + o1 = evalWith(s1, i1).
+-- + s2 = carryWith(s1, i1)
 
 inductive Vars (σ : Type) (ι : Type) (n : Nat)
-| state (s : σ)
+| state (s : Inputs σ (n + 1))
 | inputs (is : Inputs ι n)
+| outputs (os : Fin n) -- there is one output bit for each step.
 deriving DecidableEq, Hashable
 
+/--
+A state variable for the initial state.
+-/
+def Vars.state0 (s : σ) {n : Nat} : Vars σ ι n :=
+  .state (Inputs.mk ⟨0, by omega⟩ s)
+
+def Vars.stateN (s : σ) (i : Nat) {n : Nat} (hin : i ≤ n := by omega) : Vars σ ι n :=
+  .state (Inputs.mk ⟨i, by omega⟩ s)
+
+def Vars.inputN (inp : ι) (k : Nat) {n : Nat} (hkn : k < n := by omega) : Vars σ ι n :=
+  .inputs (Inputs.mk ⟨k, by omega⟩ inp)
+
+
 instance [Inhabited σ] : Inhabited (Vars σ ι n) where
-  default := .state (default)
+  default := .state (Inputs.mk ⟨0, by omega⟩ default)
 
 instance  [Inhabited ι] : Inhabited (Vars σ ι (n + 1)) where
   default := .inputs (Inputs.latest default)
 
 instance [DecidableEq σ] [DecidableEq ι] [Fintype σ] [Fintype ι] : Fintype (Vars σ ι n) where
   elems :=
-    let ss : Finset σ := Finset.univ
+    let ss : Finset (Inputs σ (n + 1)) := Finset.univ
     let ss : Finset (Vars σ ι n) := ss.map ⟨Vars.state, by intros s s'; simp⟩
+
     let ii : Finset (Inputs ι n) := Finset.univ
     let ii : Finset (Vars σ ι n) := ii.map ⟨Vars.inputs, by intros ii ii'; simp⟩
-    ss ∪ ii
+
+    let oo : Finset (Fin n) := Finset.univ
+    let oo : Finset (Vars σ ι n) := oo.map ⟨Vars.outputs, by intros o o'; simp⟩
+
+    ss ∪ ii ∪ oo
   complete := by
     intros x
     simp
@@ -523,28 +530,34 @@ instance [DecidableEq σ] [DecidableEq ι] [Fintype σ] [Fintype ι] : Fintype (
 
 def Vars.format (fσ : σ → Format) (fι : ι → Format) {n : Nat} (v : Vars σ ι n) : Format :=
   match v with
-  | .state s => fσ s
+  | .state ss => ss.format fσ
   | .inputs is => is.format fι
+  | .outputs os => f!"{os}"
 
 def Vars.castLe {n m : Nat} (v : Vars σ ι n) (hnm : n ≤ m) : Vars σ ι m :=
   match v with
-  | .state s => .state s
+  | .state ss => .state (ss.castLe (by omega))
   | .inputs is => .inputs (is.castLe hnm)
+  | .outputs os =>
+    .outputs (os.castLE (by omega))
 
 def Vars.castShift {n m : Nat} (v : Vars σ ι n) (hnm : n ≤ m) : Vars σ ι m :=
   match v with
-  | .state s => .state s
+  | .state ss => .state (ss.castShift (by omega))
   | .inputs is => .inputs (is.castShift hnm)
+  | .outputs os =>
+    .outputs ⟨os.val + (m - n), by omega⟩
 
-@[simp]
-theorem Vars.castLe_state {n m : Nat} (s : σ) (hnm : n ≤ m) :
-   (Vars.state s : Vars σ ι n).castLe hnm = Vars.state s := by rfl
+-- @[simp]
+-- theorem Vars.castLe_state {n m : Nat} (s : σ) (hnm : n ≤ m) :
+--    (Vars.state s : Vars σ ι n).castLe hnm = Vars.state s := by rfl
 
 /-- casting to the same width equals vars-/
 @[simp]
 theorem Vars.castLe_eq_self {α : Type _} {n : Nat} (v : Vars α σ n) (h : n ≤ n) :
     v.castLe h = v := by
   rcases v with x | i
+  · simp [Vars.castLe]
   · simp [Vars.castLe]
   · simp [Vars.castLe]
 
@@ -554,6 +567,7 @@ theorem Vars.castLe_castLe_eq_castLe_self {α : Type _} {p q r : Nat}
   (v : Vars α σ p) (h : p ≤ q) (h' : q ≤ r) :
     (v.castLe h).castLe h' = v.castLe (by omega) := by
   rcases v with x | i
+  · simp [Vars.castLe]
   · simp [Vars.castLe]
   · simp [Vars.castLe]
 
@@ -576,96 +590,7 @@ theorem EnvOutRelated.envBool_inputs_mk_castShift_eq_envBitStream
   rw [← hEnvBitstream.envBool_inputs_mk_eq_envBitStream]
   rfl
 
-
 attribute [simp] EnvOutRelated.envBool_inputs_mk_eq_envBitStream
-
-/-- Environment with no state variables. -/
-def envBoolEmpty_of_envBitstream
-   (envBitstream : arity → BitStream)
-   (n : Nat) : Vars Empty arity (n + 1) → Bool :=
-  fun x =>
-    match x with
-    | .state s => s.elim
-    | .inputs (.mk a i) => envBitstream i a
-
-/-- Environment with chosen state variables of the FSM. -/
-def envBoolStart_of_envBitstream (p : FSM α)
-   (envBitstream : arity → BitStream)
-   (n : Nat) : Vars p.α arity (n + 1) → Bool :=
-  fun x =>
-    match x with
-    | .state s => p.initCarry s
-    | .inputs (.mk a i) => envBitstream i a
-
-/-- Environment with chosen state variables of the FSM. -/
-def envBool_of_envBitstream_of_state
-   (envBitstream : arity → BitStream)
-   (state : α → Bool)
-   (n : Nat) : Vars α arity (n + 1) → Bool :=
-  fun x =>
-    match x with
-    | .state s => state s
-    | .inputs (.mk a i) => envBitstream i a
-
-@[simp]
-theorem envBool_of_envBitstream_of_state_eq₁ {arity : Type _} {α : Type _}
-    (envBitstream : arity → BitStream) (state : α → Bool) (n : Nat)
-    (s : α) :
-    envBool_of_envBitstream_of_state envBitstream state n (.state s) = state s := rfl
-
-@[simp]
-theorem envBool_of_envBitstream_of_state_eq₂ {arity : Type _} {α : Type _}
-    (envBitstream : arity → BitStream) (state : α → Bool) (n : Nat)
-    (i : Inputs arity (n + 1)) :
-    envBool_of_envBitstream_of_state envBitstream state n (.inputs i) =
-    envBitstream i.input i.ix := rfl
-
-def Bitstream_of_envBool
-  (envBool : Vars α arity n → Bool) :
-  (arity → BitStream) :=
-  fun a =>
-    fun k =>
-      if hk : k < n
-      then envBool (.inputs (Inputs.mk ⟨k, by omega⟩ a))
-      else false
-
-/-- make the init carry of the FSM from the envBool. -/
-def initCarry_of_envBool {p : FSM α}
-  (envBool : Vars p.α arity n → Bool) :
-  p.α → Bool := fun a => envBool (.state a)
-
-@[simp]
-theorem EnvOutRelated_envBoolEmpty_of_envBitStream_of_self {arity : Type _}
-    (envBitstream : arity → BitStream) :
-    EnvOutRelated (envBoolEmpty_of_envBitstream envBitstream n) envBitstream := by
-  constructor
-  intros x i hi
-  rw [envBoolEmpty_of_envBitstream]
-
-@[simp]
-theorem EnvOutRelated_envBoolStart_of_envBitStream_of_self {arity : Type _} {α : Type _}
-    (p : FSM α) (envBitstream : arity → BitStream) :
-    EnvOutRelated (envBoolStart_of_envBitstream p envBitstream n) envBitstream := by
-  constructor
-  intros x i hi
-  rw [envBoolStart_of_envBitstream]
-
-@[simp]
-theorem EnvOutRelated_envBoolStart_ofenvBitstream_of_state_of_self
-    {arity : Type _} {α : Type _}
-    (envBitstream : arity → BitStream) (state : α → Bool) :
-    EnvOutRelated (envBool_of_envBitstream_of_state envBitstream state n) envBitstream := by
-  constructor
-  intros x i hi
-  rw [envBool_of_envBitstream_of_state]
-
-@[simp]
-theorem EnvOutRelated_self_Bitstream_of_envBool
-    (envBool : Vars α arity n → Bool) :
-    EnvOutRelated envBool (Bitstream_of_envBool envBool) := by
-  constructor
-  intros x i hi
-  simp [Bitstream_of_envBool, hi]
 
 /-- Take the 'or' of many circuits.-/
 def Circuit.bigOr {α : Type _}
@@ -746,73 +671,6 @@ theorem Circuit.eval_bigOr_eq_true_iff
   case cons a as ih =>
     simp [bigOr, ih]
 
-def Circuit.bigOr' {α : Type _}
-    (cs : List (Circuit α)) : Circuit α :=
-  go cs Circuit.fals where
-  go : List (Circuit α) → Circuit α → Circuit α
-  | [], acc => acc
-  | c :: cs, acc =>
-    go cs (c ||| acc)
--- go [a, b] fals
--- = go [b] (a ||| fals)
--- = go [] (b ||| (a ||| fals))
--- = b ||| (a ||| fals)
-
-
-@[simp]
-theorem Circuit.bigOr'.go_append_eq {α : Type _}
-    (c : Circuit α) (cs : List (Circuit α)) (acc : Circuit α):
-    Circuit.bigOr'.go (cs ++ [c]) acc = c ||| Circuit.bigOr'.go cs acc := by
-  induction cs generalizing acc
-  case nil => simp [bigOr', bigOr'.go]
-  case cons a as ih =>
-    simp [bigOr', bigOr'.go, ih]
-
-theorem Circuit.bigOr'.append_eq {α : Type _}
-    (c : Circuit α) (cs : List (Circuit α)):
-    Circuit.bigOr' (cs ++ [c]) = c ||| Circuit.bigOr' cs := by
-  simp [bigOr', bigOr'.go_append_eq]
-
-theorem Circuit.bigOr'.go_eval_eq_false_iff
-    (cs : List (Circuit α)) (acc : Circuit α) (env : α → Bool):
-    (Circuit.bigOr'.go cs acc).eval env = false ↔
-    ((∀ (c : Circuit α), c ∈ cs → c.eval env = false) ∧ acc.eval env = false) := by
-  induction cs generalizing acc
-  case nil => simp [bigOr'.go]
-  case cons a as ih =>
-    simp [bigOr', bigOr'.go, go, ih]
-    tauto
-
-theorem Circuit.bigOr'.go_eval_eq_true_iff
-    (cs : List (Circuit α)) (acc : Circuit α) (env : α → Bool):
-    (Circuit.bigOr'.go cs acc).eval env = true ↔
-    ((∃ (c : Circuit α), c ∈ cs ∧ c.eval env = true) ∨ acc.eval env = true) := by
-  induction cs generalizing acc
-  case nil => simp [bigOr'.go]
-  case cons a as ih =>
-    simp [bigOr', bigOr'.go, go, ih]
-    constructor
-    · intros h
-      rcases h with h | h | h <;> simp [h]
-    · intros h
-      rcases h with (h | h) | h <;> simp [h]
-
-theorem Circuit.eval_bigOr'eq_false_iff
-    (cs : List (Circuit α)) (env : α → Bool):
-    (Circuit.bigOr' cs).eval env = false ↔
-    (∀ (c : Circuit α), c ∈ cs → c.eval env = false) := by
-  rw [bigOr']
-  rw [Circuit.bigOr'.go_eval_eq_false_iff]
-  simp
-
-theorem Circuit.bigOr'_eval_eq_true_iff
-    (cs : List (Circuit α)) (env : α → Bool):
-    (Circuit.bigOr' cs).eval env = true ↔
-    (∃ (c : Circuit α), c ∈ cs ∧ c.eval env = true) := by
-  rw [bigOr']
-  rw [Circuit.bigOr'.go_eval_eq_true_iff]
-  simp [Circuit.eval]
-
 /-- Take the and of many circuits.-/
 def Circuit.bigAnd {α : Type _}
     (cs : List (Circuit α)) : Circuit α :=
@@ -843,541 +701,154 @@ theorem Circuit.eval_bigAnd_eq_false_iff
       exists_eq_or_imp]
     by_cases h : a.eval env <;> simp [h, ih]
 
+
+
+structure CircuitStats where
+  iter : Nat := 0
+  size : Nat := 0
+
+deriving Repr, Inhabited, DecidableEq, Hashable
+
+
+
 /--
-Make the circuit that produces the state vector after 'n' iterations.
-This needs 'n' bits of input.
--/
-def mkCarryCircuit {arity : Type _}
+Make the funtion that for a given state 's', computes `carry(states[n][s], inputs[n])`.
+--/
+def mkCarryAssignCircuitNAux {arity : Type _}
   [DecidableEq arity]
   [Fintype arity]
   [Hashable arity]
-  (p : FSM arity) (n : Nat) : p.α → Circuit (Vars Empty arity n) := fun s =>
-  match n with
-  | 0 => Circuit.ofBool (p.initCarry s)
-  | n + 1 =>
-    (p.nextBitCirc (some s)).bind fun v =>
+  (p : FSM arity) (s : p.α) (n : Nat) : Circuit (Vars p.α arity (n + 1)) :=
+    (p.nextBitCirc (some s)).map fun v =>
       match v with
-      | .inl s' => (mkCarryCircuit p n s').map fun w =>
-        match w with
-        | .state s'' => Vars.state s''
-        | .inputs i => Vars.inputs (Inputs.mk (i.ix) i.input)
-      | .inr a => Circuit.var true (Vars.inputs (Inputs.mk ⟨n, by omega⟩ a))
-
-theorem mkCarryCircuit_eval_eq {arity : Type _}
-    [DecidableEq arity]
-    [Fintype arity]
-    [Hashable arity]
-    (p : FSM arity) (n : Nat) (s : p.α)
-    (envBool : Vars Empty arity n → Bool)
-    (envBitstream : arity → BitStream)
-    (hEnvBitstream : EnvOutRelated envBool envBitstream) :
-  (mkCarryCircuit p n s).eval envBool =
-  p.carryWith (fun s => p.initCarry s) envBitstream n s := by
-  induction n generalizing s
-  case zero =>
-    simp only [mkCarryCircuit, Circuit.ofBool, FSM.carryWith_zero_eq]
-    rcases h : p.initCarry s <;> simp [h]
-  case succ m hm =>
-    simp only [mkCarryCircuit, Fin.coe_eq_castSucc, Circuit.eval_bind,
-      FSM.carryWith_initCarry_eq_carry]
-    simp only [FSM.carry, FSM.nextBit]
-    congr
-    ext x
-    rcases x with a | i
-    · simp only [Circuit.eval_map, Sum.elim_inl]
-      rw [hm]
-      · rfl
-      · -- TODO: write this as a theorem that encapsuates that environments are related
-        -- upon casting of the input.
-        constructor
-        intros x i hi
-        simp only [Fin.castSucc_mk]
-        apply hEnvBitstream.envBool_inputs_mk_eq_envBitStream
-    · simp only [Circuit.eval, ↓reduceIte, Sum.elim_inr]
-      apply hEnvBitstream.envBool_inputs_mk_eq_envBitStream
-
+        | .inl t => Vars.stateN t n
+        | .inr i => Vars.inputN i n
 
 /--
-Make the circuit that produces the state vector after 'n' iterations,
-starting with a state vector that is given by the circuit itself.
+Make the circuit that assigns the carry state:
+  `states[n+1][:] = carry(states[n][:], inputs[n][:])`.
 -/
-def mkCarryWithCircuit {arity : Type _}
+def mkCarryAssignCircuitN {arity : Type _}
   [DecidableEq arity]
   [Fintype arity]
   [Hashable arity]
-  (p : FSM arity) (n : Nat) : p.α → Circuit (Vars p.α arity n) := fun s =>
-  match n with
-  | 0 => Circuit.var true (Vars.state s)
-  | k + 1 =>
-    (p.nextBitCirc (some s)).bind fun v =>
-      match v with
-      | .inl s' => (mkCarryWithCircuit p k s').map fun w =>
-        match w with
-        | .state s'' => Vars.state s''
-        | .inputs i => Vars.inputs (Inputs.mk (i.ix) i.input)
-      | .inr a => Circuit.var true (Vars.inputs (Inputs.mk ⟨k, by omega⟩ a))
-
-/-- make the CarryWith circuit at step 0. -/
-def mkCarryWith0Circuit {arity : Type _}
-    [DecidableEq arity]
-    [Fintype arity]
-    [Hashable arity]
-    (p : FSM arity) :
-    { f : p.α → Circuit (Vars p.α arity 0) //
-      ∀ (a : p.α), Circuit.Equiv (f a) (mkCarryWithCircuit p 0 a) } :=
-  ⟨mkCarryWithCircuit p 0, by simp⟩
-
-@[simp]
-theorem eval_mkCarryWith0Circuit_eq {arity : Type _}
-    [DecidableEq arity]
-    [Fintype arity]
-    [Hashable arity]
-    (p : FSM arity) (s : p.α)
-    (envBool : Vars p.α arity 0 → Bool) :
-  ((mkCarryWith0Circuit p).val s).eval envBool = envBool (.state s) := by
-  simp only [mkCarryWith0Circuit, mkCarryWithCircuit, Circuit.eval, Circuit.var, Vars.state]
-  rcases h : envBool (Vars.state s) <;> simp [h]
+  (p : FSM arity) (n : Nat) :
+  Circuit (Vars p.α arity (n + 1)) :=
+  let carrys := FinEnum.toList p.α |>.map fun s =>
+    -- | set the variable at states[n+1] = carry(states[n], inputs[n])
+    Circuit.xor
+      (mkCarryAssignCircuitNAux p s n)
+      (Circuit.var true <| Vars.stateN s (n + 1))
+  Circuit.bigOr carrys
 
 /--
-make the CarryWith circuit for step (n+1), incrementally,
-using the carryWith circuit at step n.
+Make the circuit that assigns `states[i][:] = carry(states[i-1][:], inputs[i-1][:])`
+for all `i ≤ n`.
 -/
-def mkCarryWithSuccCircuit {arity : Type _}
-    [DecidableEq arity]
-    [Fintype arity]
-    [Hashable arity]
-    (p : FSM arity) (n : Nat)
-    (carryN : p.α → Circuit (Vars p.α arity n))
-    (hCarryN : ∀ (a : p.α), Circuit.Equiv (carryN a) (mkCarryWithCircuit p n a)) :
-    { f : p.α → Circuit (Vars p.α arity (n + 1)) //
-      ∀ (a : p.α), Circuit.Equiv (f a) (mkCarryWithCircuit p (n + 1) a) } where
-  val := fun s =>
-    (p.nextBitCirc (some s)).bind fun v =>
-      match v with
-      | .inl s' => (carryN s').map fun w =>
-        match w with
-        | .state s'' => Vars.state s''
-        | .inputs i => Vars.inputs (Inputs.mk (i.ix) i.input)
-      | .inr a => Circuit.var true (Vars.inputs (Inputs.mk ⟨n, by omega⟩ a))
-  property := by
-    intros a
-    ext env
-    rw [mkCarryWithCircuit]
-    simp
-    simp [Circuit.eval_bind]
-    congr 1
-    ext v
-    rcases v with a' | i
-    · simp [Circuit.eval_map]
-      rw [hCarryN]
-    · simp
-
-theorem eval_mkCarryWithCircuit_eq_carryWith {arity : Type _}
-    [DecidableEq arity]
-    [Fintype arity]
-    [Hashable arity]
-    (p : FSM arity) (n : Nat) (s : p.α)
-    (envBool : Vars p.α arity n → Bool)
-    (envBitstream : arity → BitStream)
-    (hEnvBitstream : EnvOutRelated envBool envBitstream) :
-  (mkCarryWithCircuit p n s).eval envBool =
-  p.carryWith (fun s => envBool (Vars.state s)) envBitstream n s := by
-  induction n generalizing s
-  case zero =>
-    simp only [mkCarryWithCircuit, Circuit.ofBool, FSM.carryWith_zero_eq]
-    rcases h : envBool (Vars.state s) <;> simp [h]
-  case succ m hm =>
-    simp only [mkCarryWithCircuit, Fin.coe_eq_castSucc, Circuit.eval_bind,
-      FSM.carryWith_initCarry_eq_carry]
-    congr
-    ext x
-    rcases x with a | i
-    · simp only [Circuit.eval_map, Sum.elim_inl]
-      rw [hm]
-      · rfl
-      · -- Theorem: If the environments are related, then the evaluation of the circuit
-        -- with the state vector is consistent with the evaluation of the FSM.
-        constructor
-        intros x i hi
-        simp only [Fin.castSucc_mk]
-        apply hEnvBitstream.envBool_inputs_mk_eq_envBitStream
-    · simp only [Circuit.eval, ↓reduceIte, Sum.elim_inr]
-      apply hEnvBitstream.envBool_inputs_mk_eq_envBitStream
-
-
-/-
-Make the safety circuit at index 'i',
-which runs the program at the initial state on the inputs.
-See that this fixes the state to 'Empty'.
--/
-def mkEvalWithCircuit {arity : Type _}
+def mkCarryAssignCircuitLeN {arity : Type _}
   [DecidableEq arity]
   [Fintype arity]
   [Hashable arity]
-  (p : FSM arity) (n : Nat) : (Circuit (Vars p.α arity (n+1))) :=
-  p.nextBitCirc none |>.bind fun v =>
-    match v with
-    | .inl s => (mkCarryWithCircuit p n s).map fun w =>
-      match w with
-      | .state s' => Vars.state s'
-      | .inputs i => Vars.inputs (Inputs.mk ⟨i.ix, by omega⟩ i.input)
-    | .inr a => Circuit.var true (Vars.inputs (Inputs.mk ⟨n, by omega⟩ a))
-
-/-- Make the circuit that evaluates to the initial state. -/
-def mkEvalWithCircuit_of_mkCarryWithCircuit {arity : Type _}
-    [DecidableEq arity]
-    [Fintype arity]
-    [Hashable arity]
-    (p : FSM arity) (n : Nat)
-    (carryN : p.α → Circuit (Vars p.α arity n))
-    (hCarryN : ∀ (a : p.α), Circuit.Equiv (carryN a) (mkCarryWithCircuit p n a)) :
-    { c : Circuit (Vars p.α arity (n + 1)) //
-      Circuit.Equiv c (mkEvalWithCircuit p n) } where
-  val :=   p.nextBitCirc none |>.bind fun v =>
-    match v with
-    | .inl s => (carryN s).map fun w =>
-      match w with
-      | .state s' => Vars.state s'
-      | .inputs i => Vars.inputs (Inputs.mk ⟨i.ix, by omega⟩ i.input)
-    | .inr a => Circuit.var true (Vars.inputs (Inputs.mk ⟨n, by omega⟩ a))
-  property := by
-    ext v
-    rw [mkEvalWithCircuit]
-    simp [Circuit.eval_bind]
-    congr
-    ext x
-    rcases x with a | i
-    · simp [Circuit.eval_map]
-      rw [hCarryN]
-    · simp
-
-@[simp]
-theorem eval_mkEvalWithCircuit_eq
-    {arity : Type _}
-    [DecidableEq arity]
-    [Fintype arity]
-    [Hashable arity]
-    (p : FSM arity) (n : Nat)
-    (envBool : Vars p.α arity (n + 1) → Bool)
-    (envBitstream : arity → BitStream)
-    (hEnvBitstream : EnvOutRelated envBool envBitstream) :
-    (mkEvalWithCircuit p n).eval envBool =
-    p.evalWith (fun s => envBool (.state s)) envBitstream n := by
-  simp [mkEvalWithCircuit]
-  simp [Circuit.eval_bind, Circuit.eval_map]
-  rw [FSM.evalWith, FSM.eval, FSM.nextBit]
-  simp
-  congr
-  ext x
-  rcases x with a | i
-  · simp [Circuit.eval_map, Sum.elim_inl]
-    rw [eval_mkCarryWithCircuit_eq_carryWith]
-    · rw [FSM.carryWith]
-    · -- TODO extract out into generic theory.
-      constructor
-      intros x j hj
-      simp only [Fin.castSucc_mk]
-      apply hEnvBitstream.envBool_inputs_mk_eq_envBitStream
-  · simp only [Circuit.eval_map, Sum.elim_inr]
-    simp only [Circuit.eval, ↓reduceIte]
-    apply hEnvBitstream.envBool_inputs_mk_eq_envBitStream
-
-
-def mkEvalWithNCircuitAuxList {arity : Type _}
-  [DecidableEq arity] [Fintype arity] [Hashable arity]
-  (p : FSM arity) (n : Nat) : List (Circuit (Vars p.α arity (n+1))) :=
-  let ys := (List.range (n+1)).attach
-  ys.map fun i =>
-    (mkEvalWithCircuit p i.val).map (fun vs => vs.castLe (by
-      have := i.property; simp at this; omega
-    ))
-
-def mkEvalWithNCircuit {arity : Type _}
-  [DecidableEq arity] [Fintype arity] [Hashable arity]
-  (p : FSM arity) (n : Nat) : Circuit (Vars p.α arity (n+1)) :=
-  Circuit.bigOr (mkEvalWithNCircuitAuxList p n)
-
-/-- mkEvalWithNCircuit evaluated at (n + 1) equals
-mkEvalWithNCircuit evaluated at n, or'd with
-mkEvalWithCircuit evaluated at (n + 1). -/
-theorem mkEvalWithNCircuit_succ_Eqiv_mkEvalWithNCircuit_or {arity : Type _}
-    [DecidableEq arity] [Fintype arity] [Hashable arity]
-    (p : FSM arity) (n : Nat) :
-    Circuit.Equiv
-      (mkEvalWithNCircuit p (n + 1))
-      ((mkEvalWithNCircuit p n).map (fun v => v.castLe (by omega)) ||| (mkEvalWithCircuit p (n + 1))) := by
-  simp [mkEvalWithNCircuit, mkEvalWithNCircuitAuxList]
-  ext env
-  rw [NNF.bool_eq_iff]
-  rw [Circuit.eval_bigOr_eq_true_iff]
-  simp [Circuit.eval_map]
-  constructor
-  · intros h
-    obtain ⟨hc, a, ha⟩ := h
-    obtain ⟨i, hi⟩ := a
-    obtain ⟨j, hj⟩ := hi
-    subst hj
-    simp [Circuit.eval_map] at ha
-    by_cases hi : i = n + 1
-    · subst hi
-      right
-      rw [← ha]
-      simp
-    · left
-      exists (mkEvalWithCircuit p i).map (fun v => v.castLe (by omega))
-      constructor
-      · exists i
-        exists (by omega)
-      · simp [Circuit.eval_map, ha]
-  · intros h
-    rcases h with h | h
-    · obtain ⟨c, ⟨⟨i, hi, hc'⟩, hc⟩ ⟩ := h
-      subst hc'
-      simp [Circuit.eval_map] at hc ⊢
-      exists (mkEvalWithCircuit p i).map (fun v => v.castLe (by omega))
-      constructor
-      · exists i
-        exists (by omega)
-      · simp [Circuit.eval_map, hc]
-    · exists (mkEvalWithCircuit p (n + 1)).map (fun v => v.castLe (by omega))
-      simp [h]
-      exists (n + 1)
-      exists (by omega)
-      simp [Circuit.eval_map, h]
+  (p : FSM arity) (n : Nat) :
+  Circuit (Vars p.α arity (n + 1)) :=
+    let ixs := List.range (n + 1) |>.attach
+    let circs := ixs.map fun ⟨i, hi⟩ =>
+      mkCarryAssignCircuitN p i |>.map (fun v => v.castLe (by simp at hi; omega))
+    Circuit.bigOr circs
 
 /--
-Build the circuit of evaluation at [0..n+1],
-usig the circuit of evaluation at [0..n] and the
-circuit of evaluation at 'n+1'.
+Make the circuit that assigns `states[0][s] = initCarry[s]`.
 -/
-def mkEvalWithNCircuitSucc_of_mkEvalWithNCircuit_mkEvalWithCircuit_succ {arity : Type _}
-    [DecidableEq arity] [Fintype arity] [Hashable arity]
-    (p : FSM arity) (n : Nat)
-    (mkEvalWith : Circuit (Vars p.α arity (n + 2)))
-    (hMkEvalWith : Circuit.Equiv mkEvalWith (mkEvalWithCircuit p (n + 1)))
-    (mkEvalWithN : Circuit (Vars p.α arity (n + 1)))
-    (hMkEvalWithN : Circuit.Equiv mkEvalWithN (mkEvalWithNCircuit p n))
-     :
-    { c : Circuit (Vars p.α arity (n + 2)) //
-      Circuit.Equiv c (mkEvalWithNCircuit p (n + 1)) } where
-  val :=  mkEvalWithN.map (fun v => v.castLe (by omega)) ||| mkEvalWith
-  property := by
-    ext env
-    rw [mkEvalWithNCircuit_succ_Eqiv_mkEvalWithNCircuit_or]
-    simp [Circuit.eval_map]
-    rw [hMkEvalWithN, hMkEvalWith]
-
-@[simp]
-theorem eval_mkEvalWithNCircuit_eq_false_iff
-    {arity : Type _}
-    [DecidableEq arity]
-    [Fintype arity]
-    [Hashable arity]
-    (p : FSM arity) (n : Nat)
-    (envBool : Vars p.α arity (n + 1) → Bool)
-    (envBitstream : arity → BitStream)
-    (hEnvBitstream : EnvOutRelated envBool envBitstream) :
-    ((mkEvalWithNCircuit p n).eval envBool = false) ↔
-    (∀ i < n + 1, p.evalWith (fun s => envBool (.state s)) envBitstream i = false) := by
-  simp [mkEvalWithNCircuit, Circuit.eval_bigOr_eq_false_iff, mkEvalWithNCircuitAuxList]
-  constructor
-  · intros hc
-    intros i hi
-    specialize hc ?circ i (by omega) rfl
-    simp [Circuit.eval_map] at hc
-    rw [eval_mkEvalWithCircuit_eq (envBitstream := envBitstream)] at hc
-    · apply hc
-    · constructor
-      intros x j hj
-      apply hEnvBitstream.envBool_inputs_mk_eq_envBitStream
-  · intros h c i hi hc
-    subst hc
-    rw [Circuit.eval_map]
-    rw [eval_mkEvalWithCircuit_eq (envBitstream := envBitstream)]
-    · rw [← h i]
-      congr
-      omega
-    · constructor
-      intros a k hk
-      apply hEnvBitstream.envBool_inputs_mk_eq_envBitStream
-
-
-@[simp]
-theorem eval_mkEvalWithNCircuit_eq_true_iff
-    {arity : Type _}
-    [DecidableEq arity]
-    [Fintype arity]
-    [Hashable arity]
-    (p : FSM arity) (n : Nat)
-    (envBool : Vars p.α arity (n + 1) → Bool)
-    (envBitstream : arity → BitStream)
-    (hEnvBitstream : EnvOutRelated envBool envBitstream) :
-    ((mkEvalWithNCircuit p n).eval envBool = true) ↔
-    (∃ i < n + 1, p.evalWith (fun s => envBool (.state s)) envBitstream i = true) := by
-    rw [show ((mkEvalWithNCircuit p n).eval envBool = true) =
-        ¬ ((mkEvalWithNCircuit p n).eval envBool = false) by simp]
-    rw [show ∃ i < n + 1, p.evalWith (fun s => envBool (.state s)) envBitstream i = true =
-        ¬ (∀ i < n + 1, p.evalWith (fun s => envBool (.state s)) envBitstream i = false) by simp]
-    apply Iff.not
-    apply eval_mkEvalWithNCircuit_eq_false_iff (hEnvBitstream := hEnvBitstream)
+def mkInitCarryAssignCircuitAux {arity : Type _}
+  [DecidableEq arity]
+  [Fintype arity]
+  [Hashable arity]
+  (p : FSM arity) (s : p.α):
+  Circuit (Vars p.α arity 0) :=
+    Circuit.xor
+      (Circuit.ofBool (p.initCarry s))
+      (Circuit.var true <| Vars.stateN s 0)
 
 /--
-Make the circuit that sets the state vector to be the init carry of the FSM.
+Make the circuit that assigns `states[0][:] = initCarry[:]`.
 -/
-def mkCircuitWithInitCarry {arity : Type _}
-    [DecidableEq arity]
-    [Fintype arity]
-    [Hashable arity]
-    (p : FSM arity) {n : Nat} (evalCirc : Circuit (Vars p.α arity n)) : Circuit (Vars Empty arity n) :=
-  evalCirc.bind fun v =>
-    match v with
-    | .state s => Circuit.ofBool (p.initCarry s)
-    | .inputs i => Circuit.var true (Vars.inputs i)
+def mkInitCarryAssignCircuit {arity : Type _}
+  [DecidableEq arity]
+  [Fintype arity]
+  [Hashable arity]
+  (p : FSM arity) :
+  Circuit (Vars p.α arity 0) :=
+    let carrys := FinEnum.toList p.α |>.map (mkInitCarryAssignCircuitAux p)
+    Circuit.bigOr carrys
 
-/-- Show how 'mkCircuitWithInitCarry' evaluates the circuit with respect to an
-arbitrary environment: It substitutes the state vector with the initCarry,
-and leaves other data alone. -/
-@[simp]
-theorem mkCircuitWithInitCarry_eval_eq {arity : Type _}
-    [DecidableEq arity]
-    [Fintype arity]
-    [Hashable arity]
-    (p : FSM arity) {n : Nat}
-    (evalCirc : Circuit (Vars p.α arity n))
-    (envBool : Vars Empty arity n → Bool) :
-  (mkCircuitWithInitCarry p evalCirc).eval envBool =
-  evalCirc.eval (fun v =>
-    match v with
-    | .state s => p.initCarry s
-    | .inputs i => envBool (.inputs i)) := by
-  simp [mkCircuitWithInitCarry]
-  simp [Circuit.eval_bind, Circuit.eval_map]
-  congr
-  funext x
-  rcases x with a | i
-  · simp only [Circuit.eval, ↓reduceIte, Vars.state]
-    rcases p.initCarry a <;> simp
-  · simp only [Circuit.eval, ↓reduceIte, Vars.inputs]
+/--
+Make a circuit that computes `out(states[n][:], inputs[n][:])`.
+-/
+def mkOutputAssignCircuitNAux {arity : Type _}
+  [DecidableEq arity]
+  [Fintype arity]
+  [Hashable arity]
+  (p : FSM arity) (n : Nat) : Circuit (Vars p.α arity (n + 1)) :=
+    (p.nextBitCirc none).map fun v =>
+      match v with
+        | .inl s' => Vars.stateN s' n
+        | .inr i => Vars.inputN i n
+
+/-- Make a circuit that assigns
+`out[n] = out(states[n][:], inputs[n][:])`.
+-/
+def mkOutputAssignCircuitN {arity : Type _}
+  [DecidableEq arity]
+  [Fintype arity]
+  [Hashable arity]
+  (p : FSM arity) (n : Nat) :
+  Circuit (Vars p.α arity (n + 1)) :=
+    Circuit.xor
+      (mkOutputAssignCircuitNAux p n)
+      (Circuit.var true <| Vars.outputs ⟨n, by omega⟩)
+
+
+def mkOutputAssignCircuitLeN {arity : Type _}
+  [DecidableEq arity]
+  [Fintype arity]
+  [Hashable arity]
+  (p : FSM arity) (n : Nat) :
+  Circuit (Vars p.α arity (n + 1)) :=
+    let ixs := List.range (n + 1) |>.attach
+    let circs := ixs.map fun ⟨i, hi⟩ =>
+      mkOutputAssignCircuitN p i |>.map (fun v => v.castLe (by simp at hi; omega))
+    Circuit.bigOr circs
 
 
 /--
-Make the circuit that evaluates the FSM at step 'n',
-in terms of 'mkEvalWithCircuit'.
+Make a circuit that checks `out[n] = fals`.
 -/
-def mkEvalCircuit' {arity : Type _}
-    [DecidableEq arity]
-    [Fintype arity]
-    [Hashable arity]
-    (p : FSM arity) (n : Nat) :
-    Circuit (Vars Empty arity (n + 1)) :=
-  mkCircuitWithInitCarry p (mkEvalWithCircuit p n)
+def mkOutEqZeroCircuitN {arity : Type _}
+  [DecidableEq arity]
+  [Fintype arity]
+  [Hashable arity]
+  (p : FSM arity) (n : Nat) :
+  Circuit (Vars p.α arity (n + 1)) :=
+    -- | f f f
+    -- | t t f
+    Circuit.xor
+      (Circuit.ofBool false)
+      (Circuit.var true <| Vars.outputs ⟨n, by omega⟩)
+
 
 /--
-we show that `mkEvalCircuit'` equals
+Make a circuit that checks `out[n] = fals` for all `i ≤ n`
 -/
-@[simp]
-theorem eval_mkEvalCircuit'_eq
-    {arity : Type _}
-    [DecidableEq arity]
-    [Fintype arity]
-    [Hashable arity]
-    (p : FSM arity) (n : Nat)
-    (envBool : Vars Empty arity (n + 1) → Bool)
-    (envBitstream : arity → BitStream)
-    (hEnvBitstream : EnvOutRelated envBool envBitstream) :
-    -- Make a safety circuit, that computes the evaluation of the FSM.
-    (mkEvalCircuit' p n).eval envBool =
-      p.eval envBitstream n  := by
-  simp [mkEvalCircuit']
-  rw [eval_mkEvalWithCircuit_eq (envBitstream := envBitstream)]
-  · rw [FSM.evalWith_eq_eval_of_eq_init]
-    funext x
-    simp
-  · constructor
-    intros x i hi
-    simp only [Fin.castSucc_mk]
-    apply hEnvBitstream.envBool_inputs_mk_eq_envBitStream
-
-/-- Make the list of safety circuits upto length 'n + 1'. -/
-def mkSafetyCircuitAuxList {arity : Type _}
-    [DecidableEq arity]
-    [Fintype arity]
-    [Hashable arity]
-    (p : FSM arity) (n : Nat) :
-    List (Circuit (Vars Empty arity (n+1))) :=
-  let ys := (List.range (n+1)).attach
-  ys.map fun i =>
-    (mkEvalCircuit' p i.val).map (fun vs => vs.castLe (by
-      have := i.property; simp at this; omega
-    ))
-
-/--
-the circuit that witnesses safety for (n+1),
-by building an arbitrary safety circuit, and
-then using the carry circuit to set the state vector.
--/
-def mkSafetyCircuit' {arity : Type _}
-    [DecidableEq arity] [Fintype arity] [Hashable arity]
-    (p : FSM arity) (n : Nat) :
-    Circuit (Vars Empty arity (n + 1)) :=
-  mkCircuitWithInitCarry p (mkEvalWithNCircuit p n)
-
-/--
-This tells us that mkSafetyCircuit' evaluates to false
-iff the underlying FSM is unsafe up to n steps.
--/
-theorem eval_mkSafetyCircuit'_eq_false_iff_ {arity : Type _}
-    [DecidableEq arity] [Fintype arity] [Hashable arity]
-    (p : FSM arity) (n : Nat)
-    (envBool : Vars Empty arity (n + 1) → Bool)
-    (envBitstream : arity → BitStream)
-    (hEnvBitstream : EnvOutRelated envBool envBitstream) :
-    (mkSafetyCircuit' p n).eval envBool = false ↔
-    (∀ i ≤ n, p.eval envBitstream i = false) := by
-  rw [mkSafetyCircuit']
-  rw [mkCircuitWithInitCarry_eval_eq]
-  rw [eval_mkEvalWithNCircuit_eq_false_iff]
-  constructor
-  · intros h i hi
-    apply h
-    omega
-  · intros hCirc i hi
-    apply hCirc
-    omega
-  · constructor
-    intros x j hj
-    apply hEnvBitstream.envBool_inputs_mk_eq_envBitStream
-
-@[simp]
-theorem mkSafetyCircuit'_eval_eq_false_iff {arity : Type _}
-    [DecidableEq arity] [Fintype arity] [Hashable arity]
-    (p : FSM arity) (n : Nat) :
-    (∀ envBool, (mkSafetyCircuit' p n).eval envBool = false) ↔
-    (∀ envBitstream, ∀ i ≤ n, p.eval envBitstream i = false) := by
-  constructor
-  · intros h envBitstream i hi
-    let envBool := envBoolEmpty_of_envBitstream envBitstream n
-    specialize h envBool
-    rw [eval_mkSafetyCircuit'_eq_false_iff_
-      (envBitstream := envBitstream)
-    ] at h
-    · apply h
-      omega
-    · simp [envBool]
-  · intros hCirc envBool
-    rw [eval_mkSafetyCircuit'_eq_false_iff_
-      (envBitstream := Bitstream_of_envBool envBool)
-    ]
-    · intros i hi
-      apply hCirc (Bitstream_of_envBool envBool) i hi
-    · simp
-
-/-! ## Arbitrary State Vector Builder
-
-This section builds a circuit that produces the state vector after 'n' iterations,
-starting with a state vector that is given by the circuit itself.
-
--/
+def mkOutEqZeroCircuitLeN {arity : Type _}
+  [DecidableEq arity]
+  [Fintype arity]
+  [Hashable arity]
+  (p : FSM arity) (n : Nat) :
+  Circuit (Vars p.α arity (n + 1)) :=
+    let ixs := List.range (n + 1) |>.attach
+    let circs := ixs.map fun ⟨i, hi⟩ =>
+      mkOutEqZeroCircuitN p i |>.map (fun v => v.castLe (by simp at hi; omega))
+    Circuit.bigOr circs
 
 def mkUnsatImpliesCircuit (lhs rhs : Circuit α) : Circuit α :=
   -- truth table of this circuit:
@@ -1396,43 +867,6 @@ theorem mkUnsatImpliesCircuit_eq_false_iff
     (Circuit.eval lhs env = false → Circuit.eval rhs env = false) := by
   rw [mkUnsatImpliesCircuit]
   simp
-
-def mkIndHypCircuit {arity : Type _}
-  [DecidableEq arity]
-  [Fintype arity]
-  [Hashable arity]
-  (p : FSM arity) (n : Nat) : Circuit (Vars p.α arity (n+2)) :=
-  -- truth table of this circuit:
-  -- safe upto n | safe upto n+1 | output
-  --   0         |  0            | 0
-  --   0         |  1            | 1
-  --   1         |  0            | 0
-  --   1         |  1            | 0
-  mkUnsatImpliesCircuit
-    ((mkEvalWithNCircuit p n).map (fun vs => vs.castLe (by omega)))
-    (mkEvalWithCircuit p (n + 1))
-
-/-- Make a circuit that checks if two states are equal. -/
-def mkStateEqCircuit
-  {arity : Type _} {i : Nat}
-  [DecidableEq arity] [Fintype arity] [Hashable arity]
-  (p : FSM arity) (s t : p.α → Circuit (Vars p.α arity i)) : Circuit (Vars p.α arity i) :=
-  Circuit.bigOr <| FinEnum.toList p.α |>.map fun a => (s a) ^^^ (t a)
-
-
-/-- if the state circuit is false, then the states are equal under all evaluations. -/
-theorem mkStateEqCircuit_eq_zero_iff {arity : Type _} {i : Nat}
-  [DecidableEq arity] [Fintype arity] [Hashable arity]
-  (p : FSM arity) (s t : p.α → Circuit (Vars p.α arity i)) :
-  (∀ envBool, (mkStateEqCircuit p s t).eval envBool = false) ↔
-  (∀ (a : p.α) (envBool : Vars p.α arity i → Bool), (s a).eval envBool = (t a).eval envBool) := by
-  simp [mkStateEqCircuit, Circuit.eval_bigOr_eq_false_iff]
-  constructor
-  · intros h a envBool
-    apply h
-  · intros h envBool a
-    apply h
-
 
 /-- Make a circuit that checks if two states are disequal. -/
 def mkStateNeqCircuit
@@ -1463,177 +897,6 @@ theorem mkStateNeqCircuit_eq_false_iff₂  {arity : Type _} {i : Nat}
   simp [mkStateNeqCircuit, Circuit.eval_bigAnd_eq_false_iff]
 
 /--
-make the circuit that witnesses that the states are unique *after* taking 'i+1' inputs.
-We take 'i+1' so that we take at least one input.
-This circuit produces false iff...
--/
-def mkUniqueStateCircuitAux {arity : Type _}
-  [DecidableEq arity] [Fintype arity] [Hashable arity]
-  (p : FSM arity) (i : Nat) : Circuit (Vars p.α arity (i+1)) :=
-   let ins := mkCarryWith0Circuit p |>.val
-   let outs := mkCarryWithCircuit p (i+1)
-   (mkStateNeqCircuit p outs (fun s => (ins s).map  (fun v => v.castLe (by omega))))
-
-
-@[simp]
-theorem mkUniqueStateCircuitAux_eq_false_iff {arity : Type _}
-  [DecidableEq arity] [Fintype arity] [Hashable arity]
-  (p : FSM arity) (i : Nat) :
-  (∀ (envBool : Vars p.α arity (i + 1) → Bool), (mkUniqueStateCircuitAux p i).eval envBool = false) ↔
-  (∀ (envBitstream : arity → BitStream) (state : p.α → Bool) , ¬ (p.carryWith state envBitstream (i + 1) = state)) := by
-  simp [mkUniqueStateCircuitAux, mkStateEqCircuit_eq_zero_iff]
-  constructor
-  · intros h envBitstream state
-    let envBool := envBool_of_envBitstream_of_state envBitstream state i
-    specialize h envBool
-    apply Function.ne_iff.mpr
-    obtain ⟨a, ha⟩ := h
-    exists a
-    simp only [mkCarryWith0Circuit] at ha
-    simp only [Circuit.eval_map, Circuit.eval, ↓reduceIte, Vars.castLe_state] at ha
-    rw [eval_mkCarryWithCircuit_eq_carryWith (envBitstream := envBitstream)] at ha
-    · apply ha
-    · simp [envBool]
-  · intros h envBool
-    let envBitstream := Bitstream_of_envBool envBool
-    let state := fun s => envBool (.state s)
-    specialize h envBitstream state
-    have := Function.ne_iff.mp h
-    obtain ⟨a, ha⟩ := this
-    exists a
-    rw [Circuit.eval_map, eval_mkCarryWith0Circuit_eq]
-    rw [eval_mkCarryWithCircuit_eq_carryWith (envBitstream := envBitstream)]
-    · simp only [Vars.castLe_state]
-      apply ha
-    · simp [envBitstream]
-
-
-@[simp]
-theorem mkUniqueStateCircuitAux_eq_false_iff_of_EnvOutRelated {arity : Type _}
-    [DecidableEq arity] [Fintype arity] [Hashable arity]
-    (p : FSM arity) (i : Nat)
-    (envBool : Vars p.α arity (i + 1) → Bool)
-    (envBitstream : arity → BitStream)
-    (hEnvBitstream : EnvOutRelated envBool envBitstream) :
-    (((mkUniqueStateCircuitAux p i).eval envBool = false) ↔
-      ¬ (p.carryWith (fun s => envBool (.state s)) envBitstream (i + 1) = (fun s => envBool (.state s)))) := by
-  constructor
-  · intros h
-    let state := fun s => envBool (.state s)
-    apply Function.ne_iff.mpr
-    simp at h
-    rw [mkUniqueStateCircuitAux] at h
-    simp at h
-    obtain ⟨a, ha⟩ := h
-    exists a
-    rw [eval_mkCarryWithCircuit_eq_carryWith] at ha
-    rw [Circuit.eval_map] at ha
-    rw [eval_mkCarryWith0Circuit_eq] at ha
-    simp only [Circuit.eval_map, Circuit.eval, ↓reduceIte, Vars.castLe_state] at ha
-    · apply ha
-    · apply hEnvBitstream
-  · intros h
-    have := Function.ne_iff.mp h
-    obtain ⟨a, ha⟩ := this
-    rw [mkUniqueStateCircuitAux]
-    simp
-    exists a
-    rw [Circuit.eval_map, eval_mkCarryWith0Circuit_eq]
-    rw [eval_mkCarryWithCircuit_eq_carryWith (envBitstream := envBitstream)]
-    · simp only [Vars.castLe_state]
-      apply ha
-    · apply hEnvBitstream
-
-/--
-make the circuit that witnesses that the states are unique *after* taking 'i+1' inputs.
-This circuit produce false iff there are two states that are equal in [1..i+1] inputs
--/
-def mkUniqueStatesCircuit {arity : Type _}
-  [DecidableEq arity] [Fintype arity] [Hashable arity]
-  (p : FSM arity) (i : Nat) : Circuit (Vars p.α arity (i+1)) :=
-  let xs := List.range (i + 1) |>.attach
-  Circuit.bigOr <| xs.map fun j =>
-    (mkUniqueStateCircuitAux p j.val).map (fun v =>
-      v.castLe (by have := j.property; simp at this; omega))
-
-
-@[simp]
-theorem mkUniqueStatesCircuit_eq_false_iff_of_EnvOutRelated {arity : Type _}
-  [DecidableEq arity] [Fintype arity] [Hashable arity]
-  (p : FSM arity) (i : Nat)
-  (envBool : Vars p.α arity (i + 1) → Bool)
-  (envBitstream : arity → BitStream)
-  (hEnvBitstream : EnvOutRelated envBool envBitstream) :
-  ((mkUniqueStatesCircuit p i).eval envBool = false) ↔
-  (∀(j : Nat), j ≤ i →
-    ¬ (p.carryWith (fun s => envBool (.state s)) envBitstream (j + 1) =
-        (fun s => envBool (.state s)))) := by
-  simp [mkUniqueStatesCircuit, Circuit.eval_bigOr_eq_false_iff]
-  constructor
-  · intros h j hj
-    specialize h _ j (by omega) rfl
-    rw [Circuit.eval_map] at h
-    rw [mkUniqueStateCircuitAux_eq_false_iff_of_EnvOutRelated
-      (envBitstream := envBitstream)] at h
-    · simp only [Vars.castLe_state] at h
-      apply h
-    · constructor
-      intros x k hk
-      apply hEnvBitstream.envBool_inputs_mk_eq_envBitStream
-  · intros h c
-    intros j hj
-    intros hc
-    subst hc
-    rw [Circuit.eval_map]
-    rw [mkUniqueStateCircuitAux_eq_false_iff_of_EnvOutRelated
-      (envBitstream := envBitstream)]
-    · apply h j (by omega)
-    · constructor
-      intros x k hk
-      apply hEnvBitstream.envBool_inputs_mk_eq_envBitStream
-
-/-- mkUniqueStatesCircuit is false iff we don't have a repeatin state. -/
-@[simp]
-theorem mkUniqueStatesCircuit_eq_false_iff {arity : Type _}
-  [DecidableEq arity] [Fintype arity] [Hashable arity]
-  (p : FSM arity) (i : Nat) :
-  (∀ (envBool : Vars p.α arity (i + 1) → Bool), (mkUniqueStatesCircuit p i).eval envBool = false) ↔
-  (∀ (envBitstream : arity → BitStream) (state : p.α → Bool) (j : Nat),
-    j ≤ i → ¬ (p.carryWith state envBitstream (j + 1) = state)) := by
-  simp [mkUniqueStatesCircuit, Circuit.eval_bigOr_eq_false_iff]
-  constructor
-  · intros h envBitstream state
-    let envBool := envBool_of_envBitstream_of_state envBitstream state i
-    specialize h envBool
-    intros j hj
-    specialize h _ j (by omega) rfl
-    rw [Circuit.eval_map] at h
-    rw [mkUniqueStateCircuitAux_eq_false_iff_of_EnvOutRelated
-      (envBitstream := envBitstream)] at h
-    · simp only [Vars.castLe_state, envBool_of_envBitstream_of_state_eq₁, envBool] at h
-      apply h
-    · constructor
-      intros x k hk
-      rfl -- TODO: don't exploit 'rfl' here.
-  · intros h envBool
-    let envBitstream := Bitstream_of_envBool envBool
-    let state := fun s => envBool (.state s)
-    specialize h envBitstream state
-    intros c j hj hc
-    subst hc
-    rw [Circuit.eval_map]
-    rw [mkUniqueStateCircuitAux_eq_false_iff_of_EnvOutRelated
-      (envBitstream := envBitstream)]
-    · apply h j (by omega)
-    · constructor
-      intros x k hk
-      simp only [Bitstream_of_envBool, envBitstream]
-      simp only [show k < i + 1 by omega, ↓reduceDIte, envBitstream]
-      rfl
-
-
-
-/--
 Make all pairs of indices (i, j) such that 0 ≤ i < j ≤ n
 -/
 def mkLowerTriangularPairs (n : Nat) : List (Nat × Nat) :=
@@ -1650,275 +913,178 @@ theorem mem_mkLowerTriangularPairs {n : Nat} (i j : Nat) :
   simp [mkLowerTriangularPairs]
   omega
 
+
 /--
-make the circuit that witnesses that the states are unique *after* taking 'i+1' inputs.
-This circuit produce false iff there are two states that are equal in [1..i+1] inputs
+make the circuit that says that the state at index 'n' is disequal from all states [0..n)
+-/
+def mkStateUniqueCircuitN {arity : Type _}
+  [DecidableEq arity] [Fintype arity] [Hashable arity]
+  (p : FSM arity) (n : Nat) : Circuit (Vars p.α arity n) :=
+  let sn : p.α → Circuit (Vars p.α arity n) := fun s =>
+    Circuit.var true (Vars.stateN s n)
+  let circs := (List.range n).attach |>.map fun ⟨i, hi⟩ =>
+    let si : p.α → Circuit (Vars p.α arity n) := fun s =>
+      Circuit.var true (Vars.stateN s i (by simp at hi; omega))
+    (mkStateNeqCircuit p si sn)
+  Circuit.bigOr circs
+
+/--
+make the circuit that witnesses that the states are unique from [0..n]
 -/
 def mkAllPairsUniqueStatesCircuit {arity : Type _}
   [DecidableEq arity] [Fintype arity] [Hashable arity]
-  (p : FSM arity) (n : Nat) : Circuit (Vars p.α arity (n+1)) :=
+  (p : FSM arity) (n : Nat) : Circuit (Vars p.α arity n) :=
   let xs := mkLowerTriangularPairs n |>.attach
   Circuit.bigOr <| xs.map fun ⟨(i, j), hij⟩ =>
-    let si : p.α → Circuit (Vars p.α arity (n+1)) := fun s =>
-      (mkCarryWithCircuit p (i + 1) s).map (fun v =>
-        v.castLe (by have := i; simp at hij; omega))
-    let sj : p.α → Circuit (Vars p.α arity (n+1)) := fun s =>
-      (mkCarryWithCircuit p (j + 1) s).map (fun v =>
-        v.castLe (by have := j; simp at hij; omega))
+    let si : p.α → Circuit (Vars p.α arity n) := fun s =>
+      Circuit.var true (Vars.stateN s i (by simp at hij; omega))
+    let sj : p.α → Circuit (Vars p.α arity n) := fun s =>
+      Circuit.var true (Vars.stateN s j (by simp at hij; omega))
     (mkStateNeqCircuit p si sj)
 
-/-
-Establishes that all states from [0..n+1] are unique.
--/
-@[simp]
-theorem mkAllPairsUniqueStatesCircuit_eq_false_iff {arity : Type _}
+
+
+/-- structure for incrementally building the k-induction circuits. -/
+structure KInductionCircuits {arity : Type _}
+  [DecidableEq arity] [Fintype arity] [Hashable arity] (fsm : FSM arity) (n : Nat) where
+  -- | Circuit that sets states[0][s] = initCarry[s].
+  cInitCarryAssignCirc : Circuit (Vars fsm.α arity 0)
+  -- | Circuit that set states[i+1]= carry(states[i], inputs[i]) upto 'n'.
+  cSuccCarryAssignCirc : Circuit (Vars fsm.α arity (n+2))
+  -- | Circuit that sets out[i] = out(states[i], inputs[i]) upto 'n'.
+  cOutAssignCirc : Circuit (Vars fsm.α arity (n + 2))
+  -- | Circuit that says that states s0..sn are disequal
+  cStatesUniqueCirc : Circuit (Vars fsm.α arity (n + 1))
+
+namespace KInductionCircuits
+
+variable {arity : Type _}
   [DecidableEq arity] [Fintype arity] [Hashable arity]
-  (p : FSM arity) (n : Nat) :
-  (∀ (envBool : Vars p.α arity (n + 1) → Bool), (mkAllPairsUniqueStatesCircuit p n).eval envBool = false) ↔
-  (∀ (envBitstream : arity → BitStream) (state : p.α → Bool)
-      (k l : Nat), k < l → l ≤ n → ¬ (p.carryWith state envBitstream (k + 1) = p.carryWith state envBitstream (l + 1))) := by
-  constructor
-  · intros h envBitstream state k l hk hl
-    let envBool := envBool_of_envBitstream_of_state envBitstream state n
-    specialize h envBool
-    simp [mkAllPairsUniqueStatesCircuit] at h
-    specialize h _ k l (by omega) rfl
-    simp [Circuit.eval_map] at h
-    obtain ⟨a, ha⟩ := h
-    intros hContra
-    simp [envBool] at ha
-    have := congr_fun hContra a
-    rw [eval_mkCarryWithCircuit_eq_carryWith (envBitstream := envBitstream)] at ha
-    · rw [eval_mkCarryWithCircuit_eq_carryWith (envBitstream := envBitstream)] at ha
-      · simp at ha
-        apply ha
-        simp [show (fun s => state s) = state by rfl]
-        apply this
-      · constructor
-        intros x j hj
-        rfl
-    · constructor
-      intros x j hj
-      rfl
-  · intros h
-    intros envBool
-    let envBitstream := Bitstream_of_envBool envBool
-    let state := fun s => envBool (.state s)
-    simp [mkAllPairsUniqueStatesCircuit]
-    intros c k l hkl hc
-    subst hc
-    simp
-    specialize h envBitstream state k l (by omega) (by omega)
-    obtain ⟨a, ha⟩ := Function.ne_iff.mp h
-    clear h
-    exists a
-    intros hContra
-    simp [Circuit.eval_map] at hContra
-    rw [eval_mkCarryWithCircuit_eq_carryWith (envBitstream := envBitstream)] at hContra
-    · rw [eval_mkCarryWithCircuit_eq_carryWith (envBitstream := envBitstream)] at hContra
-      · simp at hContra
-        apply ha
-        exact hContra
-      · simp [envBitstream]
-        constructor
-        intros x j hj
-        simp [Bitstream_of_envBool, envBitstream, show j < n + 1 by omega]
-        rfl
-    · constructor
-      intros x j hj
-      simp [Bitstream_of_envBool, envBitstream, show j < n + 1 by omega]
-      rfl
-
-/-- induction hyp circuit. -/
-theorem eval_mkIndHypCircuit_eq_false_iff_ {arity : Type _}
-  [DecidableEq arity]
-  [Fintype arity]
-  [Hashable arity]
-  (p : FSM arity) (n : Nat)
-  {envBool : Vars p.α arity (n + 2) → Bool}
-  {envBitstream : arity → BitStream}
-  (hEnvBitstream : EnvOutRelated envBool envBitstream) :
-  (mkIndHypCircuit p n).eval envBool = false ↔
-  ((∀ i < n + 1, p.evalWith (fun s => envBool (.state s)) envBitstream i = false) →
-   (p.evalWith (fun s => envBool (.state s)) envBitstream (n + 1) = false)) := by
-  rw [mkIndHypCircuit]
-  rw [mkUnsatImpliesCircuit_eq_false_iff]
-  rw [Circuit.eval_map]
-  constructor
-  · intros h hc
-    simp [eval_mkEvalWithNCircuit_eq_false_iff (hEnvBitstream := hEnvBitstream)] at h
-    rw [eval_mkEvalWithCircuit_eq (envBitstream := envBitstream)] at h
-    · apply h
-      apply eval_mkEvalWithNCircuit_eq_false_iff  .. |>.mpr
-      · apply hc
-      · constructor
-        intros a k hk
-        apply hEnvBitstream.envBool_inputs_mk_eq_envBitStream
-    · constructor
-      intros a k hk
-      apply hEnvBitstream.envBool_inputs_mk_eq_envBitStream
-  · intros h hlhs
-    rw [eval_mkEvalWithCircuit_eq (envBitstream := envBitstream)]
-    · rw [eval_mkEvalWithNCircuit_eq_false_iff (envBitstream := envBitstream)] at hlhs
-      · apply h
-        intros j hj
-        rw [← hlhs j (by omega)]
-        · congr
-      · constructor
-        intros a k hk
-        apply hEnvBitstream.envBool_inputs_mk_eq_envBitStream
-    · constructor
-      intros a k hk
-      apply hEnvBitstream.envBool_inputs_mk_eq_envBitStream
-
-@[simp]
-theorem eval_mkIndHypCircuit_eq_false_iff {arity : Type _}
-  [DecidableEq arity]
-  [Fintype arity]
-  [Hashable arity]
-  (p : FSM arity) (n : Nat) :
-  (∀ envBool, (mkIndHypCircuit p n).eval envBool = false) ↔
-  (∀ (state : p.α → Bool) (envBitstream : arity → BitStream),
-    ((∀ i ≤ n, p.evalWith state envBitstream i = false) →
-     (p.evalWith state envBitstream (n + 1) = false))) := by
-  constructor
-  · intros h
-    intros state envBitstream hlhs
-    let envBool := envBool_of_envBitstream_of_state envBitstream state (n + 1)
-    specialize h envBool
-    rw [eval_mkIndHypCircuit_eq_false_iff_] at h
-    · apply h
-      · intros k hk
-        apply hlhs
-        omega
-    · simp [envBool]
-  · intros h
-    intros envBool
-    rw [eval_mkIndHypCircuit_eq_false_iff_]
-    let envBitstream := Bitstream_of_envBool envBool
-    · intros hCirc
-      apply h (state := fun s => envBool (.state s)) envBitstream
-      intros k hk
-      apply hCirc
-      · omega
-    · simp
-
-/-- Make the circuit that breaks the cycle in the induction hypothesis. -/
-def mkIndHypCircuitCycleBreaking {arity : Type _}
-  [DecidableEq arity]
-  [Fintype arity]
-  [Hashable arity]
-  (p : FSM arity) (n : Nat) : Circuit (Vars p.α arity (n+2)) :=
-  mkUnsatImpliesCircuit
-    -- | if all states [0..n+1] are unique
-    ((mkAllPairsUniqueStatesCircuit p n).map (fun vs => vs.castLe (by omega)))
-    -- | if ind hyp holds for [0..n+1], then it holds for [0..n+2] states.
-    (mkIndHypCircuit p n)
-
-/-- induction principle with a uniform bound 'bound' in place. -/
-@[elab_as_elim]
-theorem ind_principle₂  {motive : Nat → Prop} (bound : Nat)
-  (hBase : ∀ i ≤ bound, motive i)
-  (hInd : ∀ (i : Nat),
-    bound < i →
-    ((∀ (k : Nat), k < bound → motive (i - k - 1)) → motive i)) :
-  ∀ k, motive k := by
-  intros k
-  induction k using Nat.strong_induction_on
-  case h k ihk =>
-    by_cases hK : k ≤ bound
-    · apply hBase
-      omega
-    · have : ∃ δ, k = δ + (bound) := by exists (k - (bound)); omega
-      obtain ⟨δ, hδ⟩ := this
-      subst hδ
-      apply hInd
-      omega
-      intros ε  hε
-      apply ihk
-      omega
-
-  theorem eval_eq_false_of_mkIndHypCircuit_false_of_mkSafetyCircuit_false {n : Nat}
-    {arity : Type _}
-    [DecidableEq arity]
-    [Fintype arity]
-    [Hashable arity]
-    (p : FSM arity)
-    (hs : (mkSafetyCircuit' p n).always_false)
-    (hind : (mkIndHypCircuit p n).always_false) :
-    ∀ (envBitstream : arity → BitStream) (i : Nat), p.eval envBitstream i = false := by
-  intros envBitstream i
-  simp only [Circuit.always_false_iff, Bool.not_eq_true, mkSafetyCircuit'_eval_eq_false_iff] at hs
-  simp [eval_mkIndHypCircuit_eq_false_iff] at hind
-  rw [FSM.eval_eq_evalWith_initCarry]
-  induction i using Nat.strong_induction_on
-  case h i hStrongI =>
-    induction i using ind_principle₂ n
-    case hBase i hi =>
-      apply hs
-      omega
-    case hInd j hjLt hjInd =>
-      rw [show j = (j - (n + 1)) + (n + 1) by omega]
-      rw [FSM.evalWith_add_eq_evalWith_carryWith]
-      apply hind
-      · intros i hi
-        rw [← FSM.evalWith_add_eq_evalWith_carryWith]
-        rw [show j - (n + 1)  + i = j - (n + 1 - i) by omega]
-        rw [show j - (n + 1 - i) = j - ((n - i)) - 1 by omega]
-        by_cases hi : i = 0
-        · subst hi
-          simp
-          apply hStrongI
-          omega
-        · apply hjInd
-          · omega
-          · intros k hk; apply hStrongI; omega
+  {fsm : FSM arity}
 
 /--
-info: 'ReflectVerif.BvDecide.eval_eq_false_of_mkIndHypCircuit_false_of_mkSafetyCircuit_false' depends on axioms: [propext,
- Classical.choice,
- Quot.sound]
+Cast a circuit to a larger width, by casting the variables.
 -/
-#guard_msgs in #print axioms eval_eq_false_of_mkIndHypCircuit_false_of_mkSafetyCircuit_false
+def castCircLe {n m : Nat} (c : Circuit (Vars fsm.α arity n)) (hnm : n ≤ m := by omega) :
+    Circuit (Vars fsm.α arity m) :=
+  c.map (fun v => v.castLe hnm)
 
-/-- Version that is better suited to proving. -/
-theorem eval_eq_false_of_verifyAIG_eq_of_verifyAIG_eq
-    {arity : Type _}
-    [DecidableEq arity]
-    [Fintype arity]
-    [Hashable arity]
-    {p : FSM arity}
-    (sCert : BVDecide.Frontend.LratCert)
-    (hs : verifyCircuit (mkSafetyCircuit' p n) sCert = true)
-    (indCert : BVDecide.Frontend.LratCert)
-    (hind : verifyCircuit (mkIndHypCircuit p n) indCert = true) :
-    ∀ env i, p.eval env i = false := by
-  apply eval_eq_false_of_mkIndHypCircuit_false_of_mkSafetyCircuit_false (n := n)
-  · apply always_false_of_verifyCircuit
-    exact hs
-  · apply always_false_of_verifyCircuit
-    exact hind
+/-- Make the carry circuit for the k-induction circuits. -/
+def mkZero : KInductionCircuits fsm 0 where
+  cInitCarryAssignCirc := mkInitCarryAssignCircuit fsm
+  cSuccCarryAssignCirc := mkCarryAssignCircuitLeN fsm 1
+  cOutAssignCirc := mkOutputAssignCircuitLeN fsm 1
+  cStatesUniqueCirc := mkAllPairsUniqueStatesCircuit fsm 1
 
-/-- Prove that predicate is true iff the cerritificates check out. -/
-theorem _root_.Predicate.denote_of_verifyAIG_of_verifyAIG
-    {w : Nat}
-    {vars : List (BitVec w)}
-    (p : Predicate)
-    (n : Nat)
-    (sCert : BVDecide.Frontend.LratCert)
-    (hs : verifyCircuit (mkSafetyCircuit' (predicateEvalEqFSM p).toFSM n) sCert = true)
-    (indCert : BVDecide.Frontend.LratCert)
-    (hind : verifyCircuit (mkIndHypCircuit (predicateEvalEqFSM p).toFSM n) indCert = true) :
-    p.denote w vars := by
-  apply Predicate.denote_of_eval
-  rw [← Predicate.evalFin_eq_eval p
-    (varsList := (List.map BitStream.ofBitVec vars))
-    (varsFin := fun i => (List.map BitStream.ofBitVec vars).getD i default)]
-  · rw [(predicateEvalEqFSM p).good]
-    apply eval_eq_false_of_verifyAIG_eq_of_verifyAIG_eq
-      (n := n) (sCert := sCert) (indCert := indCert) (hs := hs) (hind := hind)
-  · intros i
-    simp
+
+-- NOTE [Circuit Equivalence As a quotient]:
+-- We ideally should have a notion of `Circuit.equiv`, which says that
+-- circuits are equivalent if they denote the same function.
+--
+-- However, for now, don't bother. We change the direction we compute the `bigOr`
+-- of the circuits, so that the latest circuit is the one that is at the outermost
+-- layer of the `bigOr`. This way, we can stick a new circuit as
+-- `circUptoN+1 = circN+1 || (...circUptoN...)`.
+
+def mkSucc
+    (prev : KInductionCircuits fsm n) :
+    KInductionCircuits fsm (n + 1) :=
+  let cInitCarryAssignCirc := prev.cInitCarryAssignCirc
+  { cInitCarryAssignCirc := cInitCarryAssignCirc
+  , cSuccCarryAssignCirc :=
+      (mkCarryAssignCircuitN fsm (n + 2)) |||
+      (castCircLe prev.cSuccCarryAssignCirc)
+  , cOutAssignCirc :=
+      (mkOutputAssignCircuitN fsm (n + 2)) |||
+      (castCircLe prev.cOutAssignCirc)
+  , cStatesUniqueCirc :=
+      mkStateUniqueCircuitN fsm (n + 2) |||
+      (castCircLe prev.cStatesUniqueCirc)
+  }
+
+/--
+The precondition that assigns all
+`s[n+1] = carry(s[n], i[n])` and assigns all `o[n+1] = out(s[n], i[n])`.
+-/
+def mkSuccCarryAndOutsAssignPrecond (circs : KInductionCircuits fsm n) :
+    Circuit (Vars fsm.α arity (n + 2)) :=
+  circs.cOutAssignCirc |||
+  circs.cSuccCarryAssignCirc
+
+
+/--
+The safety circuit that checks that if `s[0]` is assigned to init carry,
+then `o[i] = fals` for all `i ≤ n`.
+-/
+def mkPostcondSafety (_circs : KInductionCircuits fsm n) :
+    Circuit (Vars fsm.α arity (n + 1)) :=
+  mkUnsatImpliesCircuit
+    -- | If the initial state is assigned to initCarry,
+    (castCircLe <| (mkInitCarryAssignCircuit fsm))
+    -- | then the output is fals for all i ≤ n.
+    (mkOutEqZeroCircuitLeN fsm n)
+
+/--
+The induction hypothesis circuit that checks that if
+the output is zero for all `i ≤ n`, then the output is zero at `i=n+1`.
+-/
+def mkPostcondIndHypNoCycleBreaking {n} (_circs : KInductionCircuits fsm n) :
+    Circuit (Vars fsm.α arity (n + 2)) :=
+  mkUnsatImpliesCircuit
+    -- | If the output is zero for all `i ≤ n`,
+    (castCircLe (mkOutEqZeroCircuitLeN fsm <| n))
+    -- | Then the output is zero at `i = n+1`
+    (mkOutEqZeroCircuitN fsm <| n+1)
+
+/--
+If the initial state `s[0] = initCarry`,
+and `states[i+1] = carry(states[i], inputs[i])` and `out[i] = out(states[i], inputs[i])`,
+then the output is zero for all `i ≤ n`.
+-/
+def mkSafetyCircuit (circs : KInductionCircuits fsm n) :
+    Circuit (Vars fsm.α arity (n + 2)) :=
+  mkUnsatImpliesCircuit
+    (mkSuccCarryAndOutsAssignPrecond circs)
+    (castCircLe <| mkPostcondSafety circs)
+
+/--
+If states[i+1] = carry(states[i], inputs[i]) and
+out[i] = out(states[i], inputs[i]),
+and `out[i] = 0` for all `i ≤ n`,
+then the output is zero at `i = n+1`.
+-/
+def mkIndHypCircuitNoCycleBreaking (circs : KInductionCircuits fsm n) :
+    Circuit (Vars fsm.α arity (n + 2)) :=
+  mkUnsatImpliesCircuit
+    (mkSuccCarryAndOutsAssignPrecond circs)
+    -- | Then the output is zero at `i = n+1`
+    (mkPostcondIndHypNoCycleBreaking circs)
+
+/--
+If states[i+1] = carry(states[i], inputs[i]) and
+out[i] = out(states[i], inputs[i]),
+and `out[i] = 0` for all `i ≤ n`,
+then the output is zero at `i = n+1`.
+-/
+def mkIndHypCycleBreaking (circs : KInductionCircuits fsm n) :
+    Circuit (Vars fsm.α arity (n + 2)) :=
+  mkUnsatImpliesCircuit
+    (mkSuccCarryAndOutsAssignPrecond circs)
+    (mkUnsatImpliesCircuit
+      (castCircLe <| circs.cStatesUniqueCirc)
+      -- | Then the output is zero at `i = n+1`
+      (mkPostcondIndHypNoCycleBreaking circs))
+
+
+def stats {arity : Type _}
+    [DecidableEq arity] [Fintype arity] [Hashable arity]
+    {fsm : FSM arity} (circs : KInductionCircuits fsm n) : CircuitStats where
+  iter := n
+  size := circs.cSuccCarryAssignCirc.size +
+    circs.cOutAssignCirc.size +
+    circs.cInitCarryAssignCirc.size
+
+end KInductionCircuits
 
 inductive DecideIfZerosOutput
 /-- Safety property fails at this iteration. -/
@@ -1941,295 +1107,19 @@ def isSuccess : DecideIfZerosOutput → Bool
   | .provenByKIndCycleBreaking .. => true
 end DecideIfZerosOutput
 
-
--- @[nospecialize]
--- partial def decideIfZerosAuxVerified {arity : Type _}
---     [DecidableEq arity] [Fintype arity] [Hashable arity]
---     (iter : Nat) (maxIter : Nat)
---     (fsm : FSM arity) :
---     TermElabM (DecideIfZerosOutput) := do
---   trace[Bits.FastVerif] s!"K-induction (iter={iter})"
---   if iter ≥ maxIter && maxIter != 0 then
---     throwError s!"ran out of iterations, quitting"
---     return .exhaustedIterations maxIter
---   let tStart ← IO.monoMsNow
---   let cSafety : Circuit (Vars Empty arity (iter+1)) := mkSafetyCircuit' fsm iter
---   let tEnd ← IO.monoMsNow
---   let tElapsedMs := (tEnd - tStart) / 1000
---   trace[Bits.FastVerif] m!"Built safety circuit in '{tElapsedMs}s'"
-
---   let formatα : fsm.α → Format := fun s => "s" ++ formatDecEqFinset s
---   let formatEmpty : Empty → Format := fun e => e.elim
---   let formatArity : arity → Format := fun i => "i" ++ formatDecEqFinset i
---   trace[Bits.FastVerif] m!"safety circuit: {formatCircuit (Vars.format formatEmpty formatArity) cSafety}"
---   let tStart ← IO.monoMsNow
---   let safetyCert? ← checkCircuitUnsatAux cSafety
---   let tEnd ← IO.monoMsNow
---   let tElapsedMs := (tEnd - tStart) / 1000
---   trace[Bits.FastVerif] m!"Checked safety property in {tElapsedMs} seconds."
---   match safetyCert? with
---   | .none =>
---     trace[Bits.FastVerif] s!"Safety property failed on initial state."
---     return .safetyFailure iter
---   | .some safetyCert =>
---     trace[Bits.FastVerif] s!"Safety property succeeded on initial state. Building induction circuit..."
-
---     let tStart ← IO.monoMsNow
---     let cIndHyp := mkIndHypCircuit fsm iter
---     let tEnd ← IO.monoMsNow
---     let tElapsedMs := (tEnd - tStart) / 1000
---     trace[Bits.FastVerif] m!"Built induction circuit in '{tElapsedMs}s'"
-
---     let tStart ← IO.monoMsNow
---     trace[Bits.FastVerif] m!"induction circuit: {formatCircuit (Vars.format formatα formatArity) cIndHyp}"
---     -- let le : Bool := sorry
---     let indCert? ← checkCircuitUnsatAux cIndHyp
---     let tEnd ← IO.monoMsNow
---     let tElapsedMs := (tEnd - tStart) / 1000
---     trace[Bits.FastVerif] s!"Checked inductive invariant in '{tElapsedMs}s'."
---     match indCert? with
---     | .some indCert =>
---       trace[Bits.FastVerif] s!"Inductive invariant established."
---       return .proven iter safetyCert indCert
---     | .none =>
---       trace[Bits.FastVerif] s!"Unable to establish inductive invariant. Trying next iteration ({iter+1})..."
---       decideIfZerosAuxVerified (iter + 1) maxIter fsm
-
-structure CircuitStats where
-  safetySize : Nat := 0
-  indSize : Nat := 0
-deriving Repr, Inhabited, DecidableEq, Hashable
-
-/-- structure for incrementally building the k-induction circuits. -/
-structure KInductionCircuits {arity : Type _}
-  [DecidableEq arity] [Fintype arity] [Hashable arity] (fsm : FSM arity) (n : Nat) where
-  cCarryWith : fsm.α → Circuit (Vars fsm.α arity n)
-  hCarryWith : ∀ (a : fsm.α),
-    Circuit.Equiv (cCarryWith a) (mkCarryWithCircuit fsm n a)
-  cEvalWithN : Circuit (Vars fsm.α arity (n + 1))
-  hEvalWithN : Circuit.Equiv cEvalWithN (mkEvalWithNCircuit fsm n)
-
-
-namespace KInductionCircuits
-
-/-- Make the carry circuit for the k-induction circuits. -/
-def mkZero {arity : Type _}
-    [DecidableEq arity] [Fintype arity] [Hashable arity]
-    (fsm : FSM arity) :
-    KInductionCircuits fsm 0 where
-  cCarryWith := mkCarryWithCircuit fsm 0
-  hCarryWith := by intros a; simp
-  cEvalWithN := mkEvalWithNCircuit fsm 0
-  hEvalWithN := by simp
-
-
-/-- make the 'carryWith' circuit of the successor, by using the current
-circuit state. -/
-def mkSuccCarryWith {arity : Type _}
-    [DecidableEq arity] [Fintype arity] [Hashable arity]
-    (fsm : FSM arity) (n : Nat)
-    (prev : KInductionCircuits fsm n) :
-    { f : fsm.α → Circuit (Vars fsm.α arity (n + 1)) //
-      ∀ (a : fsm.α), Circuit.Equiv (f a) (mkCarryWithCircuit fsm (n + 1) a) } :=
-  mkCarryWithSuccCircuit fsm n prev.cCarryWith prev.hCarryWith
-
-/--
-make the 'evalWith' circuit of the successor, by using the current
-circuit state.
--/
-def mkSuccEvalWith {arity : Type _}
-    [DecidableEq arity] [Fintype arity] [Hashable arity]
-    (fsm : FSM arity) (n : Nat)
-    (prev : KInductionCircuits fsm n) :
-    { c : Circuit (Vars fsm.α arity (n + 2)) //
-      Circuit.Equiv c (mkEvalWithCircuit fsm (n + 1)) } :=
-  let carry := mkSuccCarryWith fsm n prev
-  mkEvalWithCircuit_of_mkCarryWithCircuit fsm (n + 1)
-    carry.val carry.prop
-
-/-- make the 'evalWithN' circuit for the (n+1)th iteration. -/
-def mkSuccEvalWithN {arity : Type _}
-    [DecidableEq arity] [Fintype arity] [Hashable arity]
-    (fsm : FSM arity) (n : Nat)
-    (prev : KInductionCircuits fsm n) :
-    { c : Circuit (Vars fsm.α arity (n + 2)) //
-      Circuit.Equiv c (mkEvalWithNCircuit fsm (n + 1)) } :=
-  let c := mkSuccEvalWith fsm n prev
-  mkEvalWithNCircuitSucc_of_mkEvalWithNCircuit_mkEvalWithCircuit_succ
-    fsm n c.val c.prop prev.cEvalWithN prev.hEvalWithN
-
--- NOTE [Circuit Equivalence As a quotient]:
--- We ideally should have a notion of `Circuit.equiv`, which says that
--- circuits are equivalent if they denote the same function.
---
--- However, for now, don't bother. We change the direction we compute the `bigOr`
--- of the circuits, so that the latest circuit is the one that is at the outermost
--- layer of the `bigOr`. This way, we can stick a new circuit as
--- `circUptoN+1 = circN+1 || (...circUptoN...)`.
-
-def mkSucc {arity : Type _}
-    [DecidableEq arity] [Fintype arity] [Hashable arity]
-    (fsm : FSM arity)
-    (prev : KInductionCircuits fsm n) :
-    KInductionCircuits fsm (n + 1) :=
-  let cCarryWith := mkCarryWithSuccCircuit fsm n
-      prev.cCarryWith prev.hCarryWith
-  let hCarryWith := cCarryWith.property
-  let cEvalWithN := mkSuccEvalWithN fsm n prev
-  let hEvalWithN := cEvalWithN.property
-  { cCarryWith,
-    hCarryWith,
-    cEvalWithN,
-    hEvalWithN
-  }
-
-
-/- Make the n'th k-induction circuit family. -/
-def mkN {arity : Type _}
-    [DecidableEq arity] [Fintype arity] [Hashable arity]
-    (fsm : FSM arity) (n : Nat) :
-    KInductionCircuits fsm n :=
-    match n with
-    | 0 => mkZero fsm
-    | n + 1 => (mkN fsm n).mkSucc
-
-/-- Make the safety circuit, incrementally. -/
-def mkSafetyCircuit {arity : Type _}
-    [DecidableEq arity] [Fintype arity] [Hashable arity]
-    {fsm : FSM arity} (circs : KInductionCircuits fsm n) :
-    { c : Circuit (Vars Empty arity (n + 1)) //
-    Circuit.Equiv c (mkSafetyCircuit' fsm n) } :=
-  let circ := mkCircuitWithInitCarry fsm circs.cEvalWithN
-  ⟨circ, by
-    rw [mkSafetyCircuit']
-    subst circ
-    ext env
-    simp only [mkCircuitWithInitCarry_eval_eq]
-    rw [circs.hEvalWithN]
-  ⟩
-
-/-#
-
-## Cycle Breaking
-
-Considere a state space where 'sgood' is the initial state, with transitions 'sgood->sgood'
-where 's0' is a good state, and unreachable states 'tgood, tbad' with transitions
-'tgood->tgood' and 'tgood->tbad'.
-
-
-Now, the reachable states are only `sgood^n = sgood`, so the automata is safe.
-
-Howver, when we do k-induction, we will explore paths of the form `tgood^n → tbad`,
-which will end in a bad state for *any* n > 0, regardless of how much we increase 'n'.
-
-To rule out such cases, we only prove the IH on paths where all states are unique.
-In the previous example, we will at `k = 2`, we will decide to not explore the path `tgood^2 → tbad`,
-which then establishes the invariant that all reachable states are unique.
-This gets us "unstuck" from cycles of bad states.
--/
-
-
-/-- Make the induction hypothesis circuit, incrementally. -/
-def mkIndHypCircuit {arity : Type _}
-    [DecidableEq arity] [Fintype arity] [Hashable arity]
-    {fsm : FSM arity} (circs : KInductionCircuits fsm n) :
-    { c : Circuit (Vars fsm.α arity (n + 2)) //
-    Circuit.Equiv c (mkIndHypCircuit fsm n) } :=
-  let circ := mkUnsatImpliesCircuit
-    (circs.cEvalWithN.map (fun vs => vs.castLe (by omega)))
-    circs.mkSuccEvalWith.val
-  ⟨circ, by
-    rw [BvDecide.mkIndHypCircuit]
-    subst circ
-    ext env
-    simp [mkUnsatImpliesCircuit, Circuit.eval_map]
-    rw [circs.hEvalWithN]
-    rw [circs.mkSuccEvalWith.prop]
-  ⟩
-
-/-- Make the induction hypothesis circuit with cycle breaking, incrementally. -/
-def mkIndHypCircuitCycleBreaking {arity : Type _}
-    [DecidableEq arity] [Fintype arity] [Hashable arity]
-    {fsm : FSM arity} (circs : KInductionCircuits fsm n) :
-    { c : Circuit (Vars fsm.α arity (n + 2)) //
-    Circuit.Equiv c (mkIndHypCircuitCycleBreaking fsm n) } :=
-  let indHyp  := circs.mkIndHypCircuit
-  let circ : Circuit <| Vars fsm.α arity (n + 2) :=
-    mkUnsatImpliesCircuit
-      ((mkAllPairsUniqueStatesCircuit fsm n).map (fun v => v.castLe (by omega)))
-      indHyp.val
-  ⟨circ, by
-    simp [circ]
-    simp [BvDecide.mkIndHypCircuitCycleBreaking]
-    ext env
-    simp [mkUnsatImpliesCircuit, Circuit.eval_map]
-    rw [indHyp.property]
-  ⟩
-
-
-def stats {arity : Type _}
-    [DecidableEq arity] [Fintype arity] [Hashable arity]
-    {fsm : FSM arity} (circs : KInductionCircuits fsm n) : CircuitStats where
-  safetySize := circs.mkSafetyCircuit.val.size
-  indSize := circs.mkIndHypCircuit.val.size
-
-  theorem eval_eq_false_of_mkN_mkIndHypCircuit_false_of_mkN_mkSafetyCircuit_false {n : Nat}
-    {arity : Type _}
-    [DecidableEq arity]
-    [Fintype arity]
-    [Hashable arity]
-    (p : FSM arity)
-    (hs : (KInductionCircuits.mkN p n).mkSafetyCircuit.val.always_false)
-    (hind : (KInductionCircuits.mkN p n).mkIndHypCircuit.val.always_false) :
-    ∀ (envBitstream : arity → BitStream) (i : Nat), p.eval envBitstream i = false := by
-  apply BvDecide.eval_eq_false_of_mkIndHypCircuit_false_of_mkSafetyCircuit_false (n := n)
-  · rw [Circuit.always_false_iff] at hs hind ⊢
-    intros env
-    rw [← (mkN p n).mkSafetyCircuit.prop]
-    simp [hs env]
-  · rw [Circuit.always_false_iff] at hs hind ⊢
-    intros env
-    rw [← (mkN p n).mkIndHypCircuit.prop]
-    simp [hind env]
-
-/-- Prove that predicate is true iff the cerritificates check out. -/
-theorem _root_.Predicate.denote_of_verifyAIG_of_verifyAIG'
-    {w : Nat}
-    {vars : List (BitVec w)}
-    (p : Predicate)
-    (n : Nat)
-    (sCert : BVDecide.Frontend.LratCert)
-    (hs : verifyCircuit (mkN (predicateEvalEqFSM p).toFSM n).mkSafetyCircuit.val sCert = true)
-    (indCert : BVDecide.Frontend.LratCert)
-    (hind : verifyCircuit (mkN (predicateEvalEqFSM p).toFSM n).mkIndHypCircuit.val indCert = true) :
-    p.denote w vars := by
-  apply Predicate.denote_of_eval
-  rw [← Predicate.evalFin_eq_eval p
-    (varsList := (List.map BitStream.ofBitVec vars))
-    (varsFin := fun i => (List.map BitStream.ofBitVec vars).getD i default)]
-  · rw [(predicateEvalEqFSM p).good]
-    apply eval_eq_false_of_mkN_mkIndHypCircuit_false_of_mkN_mkSafetyCircuit_false (n := n)
-    · rw [always_false_of_verifyCircuit]
-      rw [hs]
-    · rw [always_false_of_verifyCircuit]
-      rw [hind]
-  · intros i
-    simp
-
-end KInductionCircuits
-
 @[nospecialize]
 partial def decideIfZerosAuxVerified' {arity : Type _}
     [DecidableEq arity] [Fintype arity] [Hashable arity]
     (iter : Nat) (maxIter : Nat)
     (fsm : FSM arity)
-    (circs : KInductionCircuits fsm iter) :
-    TermElabM (DecideIfZerosOutput × CircuitStats) := do
+    (circs : KInductionCircuits fsm iter)
+    (stats : Array CircuitStats) :
+    TermElabM (DecideIfZerosOutput × Array CircuitStats) := do
   withTraceNode `trace.Bits.Fast (fun _ => return s!"K-induction (iter={iter})") do
     if iter ≥ maxIter && maxIter != 0 then
-      return (.exhaustedIterations maxIter, circs.stats)
+      return (.exhaustedIterations maxIter, stats.push circs.stats)
     let tStart ← IO.monoMsNow
-    let cSafety : Circuit (Vars Empty arity (iter+1)) := circs.mkSafetyCircuit.val
+    let cSafety : Circuit (Vars fsm.α arity (iter+2)) := circs.mkSafetyCircuit
     let tEnd ← IO.monoMsNow
     let tElapsedMs := (tEnd - tStart)
     trace[Bits.FastVerif] m!"Built new safety circuit in '{tElapsedMs}ms'"
@@ -2247,52 +1137,58 @@ partial def decideIfZerosAuxVerified' {arity : Type _}
     match safetyCert? with
     | .none =>
       trace[Bits.FastVerif] s!"Safety property failed on initial state."
-      return (.safetyFailure iter, circs.stats)
+      return (.safetyFailure iter, stats.push circs.stats)
     | .some safetyCert =>
       if iter ≥ 1 + fsm.stateSpaceSize then
         trace[Bits.FastVerif] s!"Proved safety for the entire state space (state space size: {fsm.stateSpaceSize}). No need to build induction circuit."
-        return (.provenByExhaustion iter safetyCert, circs.stats)
+        return (.provenByExhaustion iter safetyCert, stats.push circs.stats)
 
       trace[Bits.FastVerif] s!"Safety property succeeded on initial state. Building induction circuit..."
       let tStart ← IO.monoMsNow
-      let cIndHyp := circs.mkIndHypCircuitCycleBreaking
+      let cIndHyp := circs.mkIndHypCycleBreaking
       let tEnd ← IO.monoMsNow
       let tElapsedMs := (tEnd - tStart)
       trace[Bits.FastVerif] m!"Built induction circuit in '{tElapsedMs}ms'"
 
       let tStart ← IO.monoMsNow
       -- trace[Bits.FastVerif] m!"induction circuit: {formatCircuit (Vars.format formatα formatArity) cIndHyp.val}"
-      trace[Bits.FastVerif] m!"induction circuit size: {cIndHyp.val.size}"
+      trace[Bits.FastVerif] m!"induction circuit size: {cIndHyp.size}"
       -- let le : Bool := sorry
-      let indCert? ← checkCircuitUnsatAux cIndHyp.val
+      let indCert? ← checkCircuitUnsatAux cIndHyp
       let tEnd ← IO.monoMsNow
       let tElapsedMs := (tEnd - tStart)
       trace[Bits.FastVerif] s!"Checked inductive invariant in '{tElapsedMs}ms'."
       match indCert? with
       | .some indCert =>
         trace[Bits.FastVerif] s!"Inductive invariant established (iter={iter})."
-        return (.provenByKIndCycleBreaking iter safetyCert indCert, circs.stats)
+        return (.provenByKIndCycleBreaking iter safetyCert indCert, stats.push circs.stats)
       | .none =>
         trace[Bits.FastVerif] s!"Unable to establish inductive invariant. Trying next iteration ({iter+1})..."
-    decideIfZerosAuxVerified' (iter + 1) maxIter fsm  circs.mkSucc
+    decideIfZerosAuxVerified' (iter + 1) maxIter fsm  circs.mkSucc (stats.push circs.stats)
 
 
 @[nospecialize]
 def _root_.FSM.decideIfZerosVerified {arity : Type _}
     [DecidableEq arity]  [Fintype arity] [Hashable arity]
     (fsm : FSM arity) (maxIter : Nat) :
-    TermElabM (DecideIfZerosOutput × CircuitStats) :=
+    TermElabM (DecideIfZerosOutput × Array CircuitStats) :=
   -- decideIfZerosM Circuit.impliesCadical fsm
   withTraceNode `trace.Bits.Fast (fun _ => return "k-induction") (collapsed := false) do
     logInfo m!"FSM state space size: {fsm.stateSpaceSize}"
-    logInfo m!"FSM transition circuit size: {fsm.circuitSize}"
-    decideIfZerosAuxVerified' 0 maxIter fsm (KInductionCircuits.mkZero fsm)
+    -- logInfo m!"FSM transition circuit size: {fsm.circuitSize}"
+    decideIfZerosAuxVerified' 0 maxIter fsm KInductionCircuits.mkZero #[]
 
 
 /--
 An axiom tracking that the safety has been proven by exhaustion of the state space.
 -/
 axiom decideIfZerosByExhaustionAx {p : Prop}  : p
+
+/--
+An axiom tracking that the safety has been proven by exhaustion of the state space.
+-/
+axiom decideIfZerosByKInductionNoCycleBreakingAx {p : Prop}  : p
+
 
 /--
 An axiom tracking that the safety has been proven by exhaustion of the state space.
